theories/properties.v
@@ -55,37 +55,68 @@ Instance threads_terminal : Terminal (list expr) := threads_terminal'.
 Definition cfg_terminal' ρ : Prop := terminal ρ.1.
 Instance cfg_terminal : Terminal (cfg bor_lang) := cfg_terminal'.
 
+Definition external (ev: event) : option event :=
+  match ev with
+  | SysCallEvt id => Some (SysCallEvt id)
+  | _ => None
+  end.
+Definition externally_equiv : relation event :=
+  λ ev1 ev2, external ev1 = external ev2.
+
 (** Thread steps *)
-(* TODO: we are ignoring fork *)
-(* τ-step has no observation. *)
+Definition thread_step (eσ1: expr * state) (ev: event) (eσ2: expr * state) efs
+  : Prop := prim_step eσ1.1 eσ1.2 [ev] eσ2.1 eσ2.2 efs.
+(* τ-step has no external observation. *)
 Inductive thread_τstep (eσ1 eσ2: expr * state) : Prop :=
-| ThreadTauStep (STEP: prim_step eσ1.1 eσ1.2 [] eσ2.1 eσ2.2 []).
-(* One true step can be led by some τ-steps. *)
-Inductive thread_onestep eσ1 o eσ2 : Prop :=
-| ThreadOneStep eσ1'
+| ThreadTauStep ev efs
+    (INTERNAL: external ev = None)
+    (STEP: thread_step eσ1 ev eσ2 efs).
+(* One step can be led by some τ-steps. ev can be either observable or not. *)
+Inductive thread_1step eσ1 ev eσ2 : Prop :=
+| Thread1Step eσ1' efs
     (TAU_STEP: rtc thread_τstep eσ1 eσ1')
-    (ONE_STEP: prim_step eσ1'.1 eσ1'.2 [o] eσ2.1 eσ2.2 []).
+    (ONE_STEP: thread_step eσ1' ev eσ2 efs).
 
 (** Configuration (threadpool) steps *)
 (* This duplicates iris.program_logic.language in order to expose a thread id *)
-Inductive step ρ1 tid κ ρ2 : Prop :=
+Inductive step ρ1 tid ev ρ2 : Prop :=
 | StepAtomic e1 σ1 e2 σ2 efs t1 t2 :
    ρ1 = (t1 ++ e1 :: t2, σ1) →
    ρ2 = (t1 ++ e2 :: t2 ++ efs, σ2) →
-   prim_step e1 σ1 κ e2 σ2 efs →
+   thread_step (e1, σ1) ev (e2, σ2) efs →
    tid = length t1 →
-   step ρ1 tid κ ρ2.
+   step ρ1 tid ev ρ2.
 
-(* τ-step has no observation and ignore tid. *)
+(* τ-step has no external observation and ignore tid. *)
 Inductive τstep ρ1 ρ2 : Prop :=
-| CfgTauStep tid (STEP: step ρ1 tid [] ρ2).
-(* One true step can be led by some τ-steps. *)
-Inductive one_step ρ1 tid o ρ2 : Prop :=
-| CfgOneStep ρ1' (TAU_STEP: rtc τstep ρ1 ρ1') (ONE_STEP: step ρ1' tid [o] ρ2).
+| CfgTauStep tid ev
+    (INTERNAL: external ev = None)
+    (STEP: step ρ1 tid ev ρ2).
+(* One step can be led by some τ-steps. ev can be either observable or not. *)
+Inductive one_step ρ1 tid ev ρ2 : Prop :=
+| CfgOneStep ρ1'
+    (TAU_STEP: rtc τstep ρ1 ρ1')
+    (ONE_STEP: step ρ1' tid ev ρ2).
 
 (** Future states,  by interference *)
 (* TODO: fix this *)
 Definition future_state : relation state := λ σ1 σ2, σ1 = σ2.
 (** State simulation *)
 (* TODO: fix this *)
-Definition sim_state : relation state := λ σ1 σ2, σ1 = σ2.
+
+Definition sim_immediate (v1 v2: immediate) :=
+  match v1, v2 with
+  | RecV _ _ _, RecV _ _ _ => v1 = v2
+  | LitV LitPoison, LitV LitPoison => True
+  | LitV (LitInt n1), LitV (LitInt n2) => n1 = n2
+  | LitV (LitLoc l1 bor1), LitV (LitLoc l2 bor2) => l1 = l2
+  | _,_ => False
+  end.
+
+Record sim_state (σ_src σ_tgt: state) := {
+  sim_state_mem_dom : dom (gset loc) σ_src.(cheap) ≡ dom (gset loc) σ_tgt.(cheap);
+  sim_state_stack_dom : dom (gset loc) σ_src.(cstk) ≡ dom (gset loc) σ_tgt.(cstk);
+  sim_state_barriers : σ_src.(cbar) = σ_tgt.(cbar);
+  sim_state_mem : ∀ l v1 v2,
+    σ_src.(cheap) !! l = Some v1 → σ_tgt.(cheap) !! l = Some v2 → sim_immediate v1 v2;
+}.
