theories/simulation.v
@@ -5,8 +5,6 @@ From stbor Require Export properties.
 
 Notation SIM_CFG := (relation (cfg bor_lang))%type.
 
-(* TODO: do we need observations more than a singleton list? *)
-(* TODO: de we need to relax the observation relation? *)
 Definition _sim (sim: SIM_CFG) (ρ1_src ρ1_tgt : cfg bor_lang) : Prop :=
   (* Wf ρ1_src → Wf ρ1_tgt → *)
   ∀ σ1_src σ1_tgt,
@@ -16,23 +14,25 @@ Definition _sim (sim: SIM_CFG) (ρ1_src ρ1_tgt : cfg bor_lang) : Prop :=
   (* σ1_src, σ1_tgt are related *)
   sim_state σ1_src σ1_tgt →
   (* (1) If `ρ1_tgt` is terminal, then `ρ1_src` terminates with τ steps. *)
-  (terminal ρ1_tgt.1 → ∃ T2_src σ2_src,
-      rtc τstep (ρ1_src.1, σ1_src) (T2_src, σ2_src) ∧
-      sim_state σ2_src σ1_tgt ∧ terminal T2_src) ∧
+  (terminal ρ1_tgt.1 → ∃ Ts2_src σ2_src,
+      rtc τstep (ρ1_src.1, σ1_src) (Ts2_src, σ2_src) ∧
+      sim_state σ2_src σ1_tgt ∧ terminal Ts2_src) ∧
   (* (2) If `ρ1_tgt` steps to `ρ2_tgt` with observation o, then exists `ρ2_src`
          s.t. `ρ1_src` steps to `ρ2_src` with observation o AND
          ρ2_src and ρ2_tgt related by sim. *)
-  (∀ ρ2_tgt tid_tgt o, one_step (ρ1_tgt.1, σ1_tgt) tid_tgt o ρ2_tgt →
-      ∃ ρ2_src tid_src, one_step (ρ1_src.1, σ1_src) tid_src o ρ2_src ∧
+  (∀ ρ2_tgt tid_tgt ev_tgt,
+    one_step (ρ1_tgt.1, σ1_tgt) tid_tgt ev_tgt ρ2_tgt → ∃ ρ2_src tid_src ev_src,
+      one_step (ρ1_src.1, σ1_src) tid_src ev_src ρ2_src ∧
+      externally_equiv ev_src ev_tgt ∧
       sim_state ρ1_src.2 ρ2_tgt.2 ∧ sim ρ2_src ρ2_tgt).
 
 Lemma _sim_monotone : monotone2 _sim.
 Proof.
   intros ρ1_src ρ1_tgt r r' TS LE σ1_src σ1_tgt WF1 WF2 FT1 FT2 SS.
   destruct (TS _ _ WF1 WF2 FT1 FT2 SS) as [TERM STEP]. split; [done|].
-  intros ρ2_tgt tid o ONE.
-  destruct (STEP _ _ _ ONE) as [ρ2_src [tid_src [ONE_src [SS2 Hr]]]].
-  exists ρ2_src, tid_src. do 2 (split; [done|]). by apply LE.
+  intros ρ2_tgt tid ev_tgt ONE.
+  destruct (STEP _ _ _ ONE) as (ρ2_src & tid_src & ev_src & ONE' & EV & SS2 & Hr).
+  exists ρ2_src, tid_src, ev_src. do 3 (split; [done|]). by apply LE.
 Qed.
 Hint Resolve _sim_monotone: paco.
 
@@ -60,9 +60,10 @@ Definition _sim_thread (sim_thread: SIM_THREAD) (sim_terminal: SIM_EXPR)
   (* (2) If `(e1_tgt, σ1_tgt)` steps to `(e2_tgt, σ2_tgt)` with observation o,
          then exists `(e2_src, σ2_src)`
          s.t. `(e1_src, σ1_src)` steps to `(e2_src, σ2_src)` with observation o *)
-  (∀ e2_tgt σ2_tgt o, thread_onestep (e1_tgt, σ1_tgt) o (e2_tgt, σ2_tgt)
-    → ∃ e2_src σ2_src,
-      thread_onestep (e1_src, σ1_src) o (e2_src, σ2_src) ∧
+  (∀ e2_tgt σ2_tgt ev_tgt efs,
+    thread_step (e1_tgt, σ1_tgt) ev_tgt (e2_tgt, σ2_tgt) efs → ∃ e2_src σ2_src ev_src,
+      thread_1step (e1_src, σ1_src) ev_src (e2_src, σ2_src) ∧
+      externally_equiv ev_src ev_tgt ∧
       sim_state σ2_src σ2_tgt ∧
       sim_thread sim_terminal e2_src σ2_src e2_tgt σ2_tgt).
 
@@ -70,9 +71,9 @@ Lemma _sim_thread_monotone : monotone5 _sim_thread.
 Proof.
   intros re ???? r r' TS LE σ1_src σ1_tgt WF1 WF2 FT1 FT2 SS.
   destruct (TS _ _ WF1 WF2 FT1 FT2 SS) as [TERM STEP]. split; [done|].
-  intros e2_tgt σ2_tgt o ONE.
-  destruct (STEP _ _ _ ONE) as (e2_src & σ2_src & ONE_src & SS' & Hr).
-  exists e2_src, σ2_src. do 2 (split; [done|]). by apply LE.
+  intros e2_tgt σ2_tgt ev_tgt efs ONE.
+  destruct (STEP _ _ _ _ ONE) as (e2_src & σ2_src & ev_src & ONE_src & EV & SS' & Hr).
+  exists e2_src, σ2_src, ev_src. do 3 (split; [done|]). by apply LE.
 Qed.
 Hint Resolve _sim_thread_monotone: paco.
 
